{
 "cells": [
  {
   "cell_type": "markdown",
   "metadata": {},
   "source": [
    "## Use mathematical induction to prove the following statements.\n",
    "\n",
    "### (a) Let $0<a_1<\\dots<a_n$, $n$ is a positive integer, and let $e_i = \\pm 1$ for $i=1,2,\\dots,n$.\n",
    "\n",
    "### Prove that $\\sum_{i=1}^n e_ia_n$ assumes at least $\\frac{n(n+1)}{2}$ distinct value as the $e_i$ range over $2^n$ possible combination of signs.\n",
    "\n",
    "### (b) Prove that $2!4!\\dots (2n)! \\geq ((n+1)!)^n$\n",
    "\n",
    "### (c) Prove that for each integer $n$ there exists a positive integer $k$ so that $(\\sqrt{2}-1)^n = \\sqrt{k}-\\sqrt{k-1}$\n",
    "\n",
    "### (d) Let $a_i \\geq 1$ for $i=1,\\dots ,n$. Prove that\n",
    "\n",
    "### $$2^{n-1}(a_1 a_2 \\dots a_n + 1) \\geq (1+a_1) \\dots (1+a_n)$$"
   ]
  },
  {
   "cell_type": "code",
   "execution_count": null,
   "metadata": {},
   "outputs": [],
   "source": []
  },
  {
   "cell_type": "markdown",
   "metadata": {},
   "source": [
    "---\n",
    "\n",
    "### (a) Let $0<a_1<\\dots<a_n$, $n$ is a positive integer, and let $e_i = \\pm 1$ for $i=1,2,\\dots,n$.\n",
    "\n",
    "### Prove that $\\sum_{i=1}^n e_i a_i$ assumes at least $\\frac{n(n+1)}{2}$ distinct value as the $e_i$ range over $2^n$ possible combination of signs.\n",
    "\n"
   ]
  },
  {
   "cell_type": "markdown",
   "metadata": {},
   "source": [
    "---\n",
    "\n",
    "For $n=1$, $|\\{\\pm a_1\\}| = 2 \\geq \\frac{1(1+1)}{2}$ be true\n",
    "\n",
    "Suppose $n=k$ be true, $|\\sum_{i=1}^{k} e_i a_i| \\geq \\frac{k(k+1)}{2}$\n",
    "\n",
    "When $n=k+1 $, $\\{\\sum_{i=1}^{k+1} e_i a_i\\} \\supseteq A \\cup \\{y_j\\}_{j=1}^k$, where\n",
    "\n",
    "$$\\begin{array}\\\\\n",
    "A    & = & \\{(\\sum_{i=1}^{k} e_i a_i) - a_{k+1}\\}\\\\\n",
    "y_j  & = & (\\underset{1\\leq i \\leq k+1, i\\neq j}{\\sum{}}a_i) - a_j\n",
    "\\end{array}\n",
    "$$\n",
    "\n",
    "we have $|A| = |\\sum_{i=1}^{k} e_i a_i| \\geq \\frac{k(k+1)}{2}$\n",
    "\n",
    "$\\{y_j\\}$ strictly decreasing since $\\{a_i\\}$ strictly increasing, hance $|\\{y_j\\}|=k$\n",
    "\n",
    "$\\{y_j\\}$ and $A$ are disjoint since\n",
    "$$\\begin{array}\\\\\n",
    "y_k & = & (\\underset{1 \\leq i \\leq k-1}{\\sum{}}a_i)+(a_{k+1}-a_k)\\\\\n",
    "    & > & (\\underset{1 \\leq i \\leq k-1}{\\sum{}}a_i)+(a_k - a_{k+1})\\\\\n",
    "    & = & \\max{(A)}\n",
    "\\end{array}\n",
    "$$\n",
    "\n",
    "That is, we have $|\\sum_{i=1}^{k+1} e_i a_i | \\geq |A| + |\\{y_j\\}| \\geq \\frac{k(k+1)}{2} + k = \\frac{(k+2)(k+1)}{2}$"
   ]
  },
  {
   "cell_type": "code",
   "execution_count": null,
   "metadata": {},
   "outputs": [],
   "source": []
  },
  {
   "cell_type": "markdown",
   "metadata": {},
   "source": [
    "---\n",
    "\n",
    "### (b) Prove that $2!4!\\dots (2n)! \\geq ((n+1)!)^n$\n",
    "\n",
    "---\n",
    "\n",
    "For $n=1$, $2!= ((1+1)!)^2$ be true\n",
    "\n",
    "Suppose $n=k$ be true, $\\underset{1\\leq i \\leq k}\\Pi{2i} \\geq ((k+1)!)^k$\n",
    "\n",
    "When $n=k+1 $, to prove this inequality, we argue $\\frac{\\text{LHS}}{\\text{RHS}} \\geq 1$\n",
    "\n",
    "$$\\begin{array}\\\\\n",
    "\\frac{\\underset{1\\leq i \\leq k+1}\\Pi{2i}}{((k+2)!)^{(k+1)} } & \\geq & \\frac{((2k+2)!)((k+1)!)^k}{((k+2)!)^{(k+1)} } \\\\\n",
    "                                                             &  =   & \\frac{((2k+2)!)((k+1)!)^k}{((k+1)!)^{k} (k+2)^k\n",
    "                                                                                                 ((k+2)!)} \\\\\n",
    "                                                             &  =   & \\frac{((2k+2)!)}{ (k+2)^k ((k+2)!)} \\\\\n",
    "                                                             &  =   & \\frac{(k+2+1)(k+2+2)\\dots (k+2+k)}{(k+2)^k}\\\\\n",
    "                                                             &  >   & 1\\\\\n",
    "\\end{array}\n",
    "$$"
   ]
  },
  {
   "cell_type": "code",
   "execution_count": null,
   "metadata": {},
   "outputs": [],
   "source": []
  },
  {
   "cell_type": "markdown",
   "metadata": {},
   "source": [
    "---\n",
    "\n",
    "### (c) Prove that for each integer $n$ there exists a positive integer $k$ so that $(\\sqrt{2}-1)^n = \\sqrt{k}-\\sqrt{k-1}$\n",
    "\n",
    "---\n",
    "\n",
    "#### Claim $(\\sqrt{2}-1)^n = (-1)^{n}\\alpha_n\\sqrt{2} + (-1)^{n-1}\\beta_n some $ for $\\alpha_n, \\beta_n$ be integers\n",
    "\n",
    "When $n=1, \\alpha=\\beta=1$ be true\n",
    "\n",
    "Suppose that $n=l$ be true. That is, $(\\sqrt{2}-1)^l = (-1)^{l}\\alpha_l\\sqrt{2} + (-1)^{l-1}\\beta_l$\n",
    "\n",
    "When $n=l+1$,\n",
    "$$\\begin{array}\\\\\n",
    "(\\sqrt{2}-1)^{l+1} & = & ((-1)^{l}\\alpha_l\\sqrt{2} + (-1)^{l-1}\\beta_l)*(\\sqrt{2}-1)\\\\\n",
    "                   & = & ((-1)^{l+1}(\\alpha_l+\\beta_l)\\sqrt{2} + (-1)^{l-1}(2\\alpha_l+\\beta_l))\\\\\n",
    "\\alpha_{l+1}       & = & \\alpha_l + \\beta_l \\\\\n",
    "\\beta_{l+1}        & = & 2\\alpha_l + \\beta_l \\\\\n",
    "\\end{array}\n",
    "$$\n",
    "\n",
    "#### Main statement\n",
    "\n",
    "When $n=1, k_1=2$ be true.\n",
    "\n",
    "Suppose that $n=l$ be true. That is, $(\\sqrt{2}-1)^l = \\sqrt{k_l}-\\sqrt{k_l - 1}$\n",
    "\n",
    "By the claim above\n",
    "$$\n",
    "k_l = \n",
    "\\begin{cases}\n",
    "2\\alpha_l^2\\text{, for $l$ even}\\\\\n",
    "\\beta_l^2\\text{, for $l$ odd}\\\\\n",
    "\\end{cases}\n",
    "$$\n",
    "\n",
    "$$\n",
    "2\\alpha_l^2 - \\beta_l^2 = (-1)^l\n",
    "$$\n",
    "\n",
    "\n",
    "When $n=l+1$,\n",
    "\n",
    "$$\\begin{array}\\\\\n",
    "2\\alpha_{l+1}^2 - \\beta_{l+1}^2 & = & (2\\alpha_l^2 + 4\\alpha_l\\beta_l + 2\\beta_l^2)\n",
    "                                        - (4\\alpha_l^2 + 4\\alpha_l\\beta_l + \\beta_l^2)\\\\\n",
    "                                & = & -(2\\alpha_l^2 - \\beta_l^2)\\\\\n",
    "                                & = & (-1)^{l+1}\n",
    "\\end{array}\n",
    "$$\n",
    "\n",
    "and then set\n",
    "\n",
    "$$\n",
    "k_{l+1} = \n",
    "\\begin{cases}\n",
    "2\\alpha_{l+1}^2\\text{, for $l+1$ even}\\\\\n",
    "\\beta_{l+1}^2\\text{, for $l+1$ odd}\\\\\n",
    "\\end{cases}\n",
    "$$\n",
    "\n",
    "we got $(\\sqrt{2}-1)^{l+1} = \\sqrt{k_{l+1}}-\\sqrt{k_{l+1} - 1}$"
   ]
  },
  {
   "cell_type": "code",
   "execution_count": null,
   "metadata": {},
   "outputs": [],
   "source": []
  },
  {
   "cell_type": "markdown",
   "metadata": {},
   "source": [
    "---\n",
    "### (d) Let $a_i \\geq 1$ for $i=1,\\dots ,n$. Prove that\n",
    "\n",
    "### $$2^{n-1}(a_1 a_2  \\dots a_n + 1) \\geq (1+a_1) \\dots (1+a_n)$$\n",
    "---\n",
    "\n",
    "For $n=1$, $(1+a_1) = (1+a_1)$ be true\n",
    "\n",
    "Suppose $n=k$ be true, $2^{k-1}(a_1 a_2 \\dots a_k + 1) \\geq (1+a_1) \\dots (1+a_k)$\n",
    "\n",
    "set\n",
    "$$\\begin{array}\\\\\n",
    "b_i & = & a_1 a_2 \\dots a_i\\\\\n",
    "c_i & = & (1+a_1) \\dots (1+a_i)\n",
    "\\end{array}\n",
    "$$\n",
    "\n",
    "get\n",
    "\n",
    "$$ 2^{k-1}(b_{k} + 1) \\geq c_{k} $$\n",
    "\n",
    "\n",
    "When $n=k+1$,\n",
    "\n",
    "$$\\begin{array}\\\\\n",
    "\\text{LHS} - \\text{RHS} &  =  & 2^{k}(b_{k+1} + 1) - c_{k+1}\\\\\n",
    "                        &  =  & 2^{k}(b_{k}a_{k+1} + 1) - c_{k}(1+a_{k+1})\\\\\n",
    "                        & \\geq& 2^{k}(b_{k}a_{k+1} + 1) - 2^{k-1}(b_{k} + 1)(a_{k+1} + 1)\n",
    "                                 &\\text{,  by the truth when $n=k$ , note minus symbol}\\\\\n",
    "                        & \\geq& p\\Big((2b_{k}a_{k+1} + 2) - (b_{k}a_{k+1} + b_k + a_{k+1} + 1) \\Big)\n",
    "                                 &\\text{, set } p =  2^{k-1}\\\\\n",
    "                        &  =  & p(b_{k}a_{k+1} - b_k - a_{k+1} + 1)\\\\\n",
    "                        &  =  & p(b_{k} - 1)(a_{k+1} - 1)\\\\\n",
    "                        & \\geq& 0\n",
    "\\end{array}\n",
    "$$\n"
   ]
  },
  {
   "cell_type": "code",
   "execution_count": null,
   "metadata": {},
   "outputs": [],
   "source": []
  }
 ],
 "metadata": {
  "kernelspec": {
   "display_name": "Python 3",
   "language": "python",
   "name": "python3"
  },
  "language_info": {
   "codemirror_mode": {
    "name": "ipython",
    "version": 3
   },
   "file_extension": ".py",
   "mimetype": "text/x-python",
   "name": "python",
   "nbconvert_exporter": "python",
   "pygments_lexer": "ipython3",
   "version": "3.7.2"
  }
 },
 "nbformat": 4,
 "nbformat_minor": 2
}
