{
 "cells": [
  {
   "cell_type": "markdown",
   "metadata": {},
   "source": [
    "## The following are a set of problems related to sets and functions.\n",
    "\n",
    "### (a) Let $\\Omega$ be a nonempty set. For $A, B \\subset \\Omega$, define there \"symmetric difference\" as $A \\circ B =(A-B)\\cup(B-A)$. Prove that for subset $A,B,C \\subset \\Omega,$\n",
    "\n",
    "### $$\\text{(1) } A \\circ (B \\circ C) = (A \\circ B) \\circ C$$\n",
    "\n",
    "### $$\\text{(2) } A \\cap (B \\circ C) = (A \\cap B) \\circ (A \\cap C)$$\n",
    "\n",
    "### Also, (3) prove that $A = \\emptyset \\iff B = B \\circ A \\text{ for all } B \\subset \\Omega$.\n",
    "\n",
    "### Finally, (4) can the equality $A \\cup (B \\circ C) = (A \\cup B) \\circ (A \\cup C)$ be ture?\n",
    "\n",
    "---\n",
    "\n",
    "### (b) Let $f : A \\rightarrow B$ be a function. $\\{ C_\\alpha \\}_{\\alpha \\in I}$ is a familly of subsets of $B$ indexed by the set $I$. Prove that\n",
    "\n",
    "### $$\\text{(1) } f^{-1}(\\cup_{\\alpha \\in I}C_\\alpha) = \\cup_{\\alpha \\in I} f^{-1}(C_\\alpha)$$\n",
    "\n",
    "### $$\\text{(2) } f^{-1}(\\cap_{\\alpha \\in I}C_\\alpha) = \\cap_{\\alpha \\in I} f^{-1}(C_\\alpha)$$\n",
    "\n",
    "### Moreover, prove that (3) $f^{-1}(B-C) = A - f^{-1}(C) \\text{ for any subset } B \\subset C$.\n",
    "\n",
    "---"
   ]
  },
  {
   "cell_type": "markdown",
   "metadata": {
    "collapsed": true
   },
   "source": [
    "---\n",
    "\n",
    "\n",
    "### (a) Let $\\Omega$ be a nonempty set. For $A, B \\subset \\Omega$, define there \"symmetric difference\" as $A\\circ B =(A-B)\\cup(B-A)$. Prove that for subset $A,B,C \\subset \\Omega,$\n",
    "\n",
    "### $$\\text{(1) } A \\circ (B \\circ C) = (A \\circ B) \\circ C$$\n",
    "\n",
    "### $$\\text{(2) } A \\cap (B \\circ C) = (A \\cap B) \\circ (A \\cap C)$$\n",
    "\n",
    "### Also, (3) prove that $A = \\emptyset \\iff B = B \\circ A \\text{ for all } B\\subset \\Omega$.\n",
    "\n",
    "### Finally, (4) can the equality $A \\cup (B \\circ C) = (A \\cup B) \\circ (A \\cup C)$ be ture?\n",
    "\n",
    "---\n",
    "\n",
    "(1)\n",
    "\n",
    "First, we have this equality, $\\forall A,B,C,D \\subset \\Omega$\n",
    "\n",
    "$$\\begin{array}\\\\\n",
    "(A \\cup B) \\cap (C \\cup D) & = & ((A \\cup B) \\cap C) \\cup ((A \\cup B) \\cap D) \\\\\n",
    "& = & (A \\cap C) \\cup (B \\cap C) \\cup (A \\cap D) \\cup (B \\cap D) & \\cdots \\cdots \\cdots \\text{(1)}\n",
    "\\end{array}\n",
    "$$\n",
    "\n",
    "Return to what we want,\n",
    "\n",
    "$$\\begin{array}\\\\\n",
    "A \\circ (B \\circ C) & = & A \\circ ((B - C) \\cup (C - B))\\\\\n",
    "                    & = & (A - ((B - C) \\cup (C - B))) \\cup (((B - C) \\cup (C - B))-A) \\\\\n",
    "                    & = & ((A-(B-C)) \\cap (A-(C-B))) \\cup (((B-C)-A) \\cup ((C - B)-A))\\\\\n",
    "                    & = & ((A \\cap (B' \\cup C)) \\cap (A \\cap (C' \\cup B))) \\cup (B \\cap C' \\cap A') \\cup (C \\cap B' \\cap A')\\\\\n",
    "                    \\\\\n",
    "                    & = & (((A \\cap B') \\cup (A \\cap C)) \\cap ((A \\cap C') \\cup (A \\cap B))) \\\\\n",
    "                    &   & \\cup (B \\cap C' \\cap A') \\\\\n",
    "                    &   & \\cup (C \\cap B' \\cap A')\\\\\n",
    "                    \\\\\n",
    "                    & = & \\cup (A \\cap B \\cap C) \\\\\n",
    "                    &   & \\cup (A \\cap B' \\cap C') \\\\\n",
    "                    &   & \\cup (B \\cap C' \\cap A') \\\\\n",
    "                    &   & \\cup (C \\cap A' \\cap B') \\text{ , apply (1)} \\\\\n",
    "                    \\\\\n",
    "                    & = & C \\circ (A \\circ B) \\text{ , since this foumula is symmetric for } A,B,C \\\\\n",
    "                    & = & (A \\circ B) \\circ C\n",
    "\\end{array}\n",
    "$$\n",
    "\n",
    "(2)\n",
    "\n",
    "$$\n",
    "\\begin{array}\\\\\n",
    "LHS & = & A \\cap (B \\circ C) \\\\\n",
    "    & = & A \\cap ((B \\cap C') \\cup (C \\cap B')) \\\\\n",
    "    & = & (A \\cap B \\cap C') \\cup (A \\cap C \\cap B') \\\\\n",
    "    \\\\\n",
    "RHS & = & ((A \\cap B) - (A \\cap C)) \\cup ((A \\cap C) - (A \\cap B)) \\\\\n",
    "    & = & ((A \\cap B \\cap (A' \\cup C')) \\cup ((A \\cap C \\cap (A' \\cup B')) \\\\\n",
    "    & = & (A \\cap B \\cap C') \\cup (A \\cap C \\cap B') \\text{ ,since } A \\cap A' = \\emptyset\\\\\n",
    "    & = & LHS\n",
    "\\end{array}\n",
    "$$\n",
    "\n",
    "(3)\n",
    "\n",
    "If $A = \\emptyset$\n",
    "\n",
    "$$\n",
    "B \\circ A = (B - \\emptyset) \\cup (\\emptyset - B) = B \\cup \\emptyset = B\n",
    "$$\n",
    "\n",
    "Otherwise, for $A \\neq \\emptyset$, pick $x \\in A$,\n",
    "\n",
    "if $x \\in B$ we have $x \\notin B - A \\text{ and } x \\notin A-B$,\n",
    "\n",
    "that is $x \\notin A \\circ B$\n",
    "\n",
    "$\\implies B \\neq A \\circ B$\n",
    "\n",
    "if $x \\notin B$, we have $x \\in (A-B) \\subset A \\circ B$ \n",
    "\n",
    "$\\implies B \\neq A \\circ B$\n",
    "\n",
    "(4)\n",
    "\n",
    "This equlity is false, for $A \\neq \\emptyset$, pick $x \\in A$ \n",
    "\n",
    "$x \\in A \\subset \\text{LHS}$\n",
    "\n",
    "but, $x \\notin $RHS because that\n",
    "\n",
    "$$\n",
    "\\begin{array}\\\\\n",
    "         & x \\in A \\cup B & \\text{ and } & x \\in A \\cup C \\\\\n",
    "\\implies & x \\notin ((A \\cup B) - (A \\cup C)) & \\text{ and } & x \\notin ((A \\cup C) - (A \\cup B))\\\\\n",
    "\\implies & x \\notin \\text{RHS}\n",
    "\\end{array}\n",
    "$$"
   ]
  },
  {
   "cell_type": "markdown",
   "metadata": {
    "collapsed": true
   },
   "source": [
    "---\n",
    "\n",
    "### (b) Let $f : A \\rightarrow B$ be a function. $\\{ C_\\alpha \\}_{\\alpha \\in I}$ is a familly of subsets of $B$ indexed by the set $I$. Prove that\n",
    "\n",
    "### $$\\text{(1) } f^{-1}(\\cup_{\\alpha \\in I}C_\\alpha) = \\cup_{\\alpha \\in I} f^{-1}(C_\\alpha)$$\n",
    "\n",
    "### $$\\text{(2) } f^{-1}(\\cap_{\\alpha \\in I}C_\\alpha) = \\cap_{\\alpha \\in I} f^{-1}(C_\\alpha)$$\n",
    "\n",
    "### Moreover, prove that (3) $f^{-1}(B-C) = A - f^{-1}(C) \\text{ for any subset } B \\subset C$.\n",
    "\n",
    "---\n",
    "\n",
    "(1)\n",
    "\n",
    "\" $\\subseteq$ \"\n",
    "\n",
    "given $x \\in $LHS, there exists $y \\in \\cup_{\\alpha \\in I}C_\\alpha$ such that $f(x) = y$\n",
    "\n",
    "$\\implies y \\in C_\\alpha \\text{ for some } \\alpha \\in I$\n",
    "\n",
    "$\\implies x \\in f^{-1}(C_\\alpha) \\text{ for some } \\alpha \\in I$\n",
    "\n",
    "$\\implies x \\in $RHS\n",
    "\n",
    "$ $\n",
    "\n",
    "\" $\\supseteq$ \"\n",
    "\n",
    "given $x \\in $RHS, there exists $y \\in C_\\alpha \\text{ for some } \\alpha \\in I$ such that $f(x) = y$\n",
    "\n",
    "$\\implies y \\in \\cup_{\\alpha \\in I}C_\\alpha$\n",
    "\n",
    "$\\implies x \\in$LHS\n",
    "\n",
    "$ $\n",
    "\n",
    "(2)\n",
    "\n",
    "\" $\\subseteq$ \"\n",
    "\n",
    "Given $x \\in $LHS, there exists $y \\in \\cap_{\\alpha \\in I}C_\\alpha$ such that $f(x) = y$\n",
    "\n",
    "$\\implies y \\in C_\\alpha \\text{ for all } \\alpha \\in I$\n",
    "\n",
    "$\\implies x \\in f^{-1}(C_\\alpha) \\text{ for all } \\alpha \\in I$\n",
    "\n",
    "$\\implies x \\in $RHS\n",
    "\n",
    "$ $\n",
    "\n",
    "\" $\\supseteq$ \"\n",
    "\n",
    "Given $x \\in $RHS, there exists $y \\in C_\\alpha \\text{ for all } \\alpha \\in I$ such that $f(x) = y$\n",
    "\n",
    "$\\implies y \\in \\cap_{\\alpha \\in I}C_\\alpha$\n",
    "\n",
    "$\\implies x \\in$LHS\n",
    "\n",
    "$ $\n",
    "\n",
    "(3)\n",
    "\n",
    "\" $\\supseteq$ \"\n",
    "\n",
    "For all $x \\in $RHS, $ f(x) = y \\in B$,\n",
    "\n",
    "but $y \\notin C$ since $x \\notin f^{-1}(C)$\n",
    "\n",
    "$\\implies y \\in B - C$\n",
    "\n",
    "$\\implies x \\in $LHS\n",
    "\n",
    "$ $\n",
    "\n",
    "\" $\\subseteq$ \"\n",
    "\n",
    "Suppose not,\n",
    "\n",
    "there exists $x \\in A, x \\in $LHS but $x \\notin$RHS\n",
    "\n",
    "$x \\notin$RHS $\\implies x \\in f^{-1}(C), \\text{ that is } f(x) \\in C$\n",
    "\n",
    "$x \\in $LHS $\\implies f(x) \\in B-C $\n",
    "\n",
    "so, we have $f(x) \\in (B-C) \\cap C = \\emptyset$, contradiction"
   ]
  },
  {
   "cell_type": "code",
   "execution_count": null,
   "metadata": {
    "collapsed": true
   },
   "outputs": [],
   "source": []
  }
 ],
 "metadata": {
  "kernelspec": {
   "display_name": "Python 3",
   "language": "python",
   "name": "python3"
  },
  "language_info": {
   "codemirror_mode": {
    "name": "ipython",
    "version": 3
   },
   "file_extension": ".py",
   "mimetype": "text/x-python",
   "name": "python",
   "nbconvert_exporter": "python",
   "pygments_lexer": "ipython3",
   "version": "3.6.1"
  }
 },
 "nbformat": 4,
 "nbformat_minor": 2
}
